progress on hash example [elton]

theories/elton/examples/hash_guess.v
@@ -1,20 +1,20 @@
+From iris.base_logic.lib Require Import token.
 From clutch.elton Require Import elton hash. 
 Set Default Proof Using "Type*".
 
-Section proofs.
-  Context `{eltonGS Σ}.
+Section prog.
   Variable secret_range:nat.
   Variable val_size: nat.
-  Variable bound: nat.
+  Variable tries: nat.
 
   Definition prog : expr :=
     λ: "A",
-      let: "hashf" := init_hash val_size in
+      let: "hashf" := init_hash val_size #() in
       let: "secret" := rand #secret_range in
       let: "h" := "hashf" "secret" in
-      let: "i" := ref #bound in
+      let: "i" := ref #tries in
       let: "hashf'" :=
-        (λ: "x", if: ! "x" = #0
+        (λ: "x", if: ! "i" = #0
                  then NONE
                  else "i" <- ! "i" - #1;; SOME ("hashf" "x") ) in
       let: "g" := "A" "hashf'" "h" in
@@ -23,16 +23,347 @@ Section proofs.
   
   Definition prog' : expr :=
     λ: "A",
-      let: "hashf" := init_hash val_size in
+      let: "hashf" := init_hash val_size #() in
       let: "secret" := drand #secret_range in
       let: "h" := "hashf" "secret" in
-      let: "i" := ref #bound in
+      let: "i" := ref #tries in
       let: "hashf'" :=
-        (λ: "x", if: ! "x" = #0
+        (λ: "x", if: ! "i" = #0
                  then NONE
                  else "i" <- ! "i" - #1;; SOME ("hashf" "x") ) in
       let: "g" := "A" "hashf'" "h" in
       "hashf" "g" = "h".
   
-End proofs.
+  (* Context `{eltonGS Σ}. *)
+
+  Lemma guess_hash A:
+    ∅ ⊢ₜ A : ((TNat → (TUnit+TNat)) → TNat → TNat) ->
+             pgl (lim_exec ((prog A), {|heap:=∅; urns:= ∅|})) (λ v, v=#false)
+               ((tries+1)%nat * (/(secret_range +1)%nat + /(val_size + 1)%nat) ).
+  Proof. 
+    intros Htyped.
+    eapply (elton_adequacy_remove_drand (#[eltonΣ; tokenΣ]) (prog' A)).
+    - simpl. by erewrite typed_remove_drand_expr.
+    - apply Rmult_le_pos; first apply pos_INR.
+      rewrite -!Rdiv_1_l.
+      apply Rplus_le_le_0_compat;
+        apply Rcomplements.Rdiv_le_0_compat; try lra.
+      all: apply lt_0_INR; lia. 
+    - rewrite /prog'.
+      iIntros (? Φ).
+      iModIntro. iIntros "Herr HΦ".
+      iPoseProof (typed_safe _ [] _ Htyped) as "H".
+      wp_bind (A).
+      iApply (pgl_wp_wand); first done.
+      iIntros (?) "#Hinterp".
+      simpl.
+      wp_pures.
+      rewrite plus_INR.
+      rewrite Rmult_plus_distr_r.
+      iDestruct (ec_split with "[$]") as "[Herr1 Herr2]".
+      { apply Rmult_le_pos; first apply pos_INR.
+        rewrite -!Rdiv_1_l.
+        apply Rplus_le_le_0_compat;
+          apply Rcomplements.Rdiv_le_0_compat; try lra.
+        all: apply lt_0_INR; lia.  }
+      { apply Rmult_le_pos; first apply pos_INR.
+        rewrite -!Rdiv_1_l.
+        apply Rplus_le_le_0_compat;
+          apply Rcomplements.Rdiv_le_0_compat; try lra.
+        all: apply lt_0_INR; lia.  }
+      wp_apply (wp_init_hash); first done.
+      iIntros (f) ">Hf".
+      wp_pures.
+      wp_apply (wp_drand_thunk _ _ _ _ _ (True)).
+      { rewrite rupd_unseal/rupd_def.
+        iIntros (?) "$".
+        iPureIntro.
+        intros.
+        simpl.
+        eexists _; split; first done.
+        f_equal.
+        f_equal. 
+        instantiate (1:=secret_range).
+        lia. }
+      iIntros (l) "[_ Hl]".
+      rewrite Nat2Z.id.
+      wp_pures.
+      iMod (ec_zero) as "Hzero".
+      wp_apply (wp_insert_new _ _ _ _ _ _ (λ _, 0)%R True with "[$Hf $Hzero]").
+      { done. }
+      { by intros. }
+      { right. apply SeriesC_0. intros. lra. }
+      { iModIntro. rewrite dom_empty_L. by rewrite big_sepS_empty. }
+      iIntros (secret) "(Hf&_)".
+      wp_pures.
+      wp_alloc lt as "Hr".
+      wp_pures.
+      iAssert (∃s, l↪urn_unif s ∗ ⌜size s = S secret_range⌝)%I with "[$Hl]" as "H'".
+      { iPureIntro.
+        rewrite size_list_to_set.
+        - rewrite length_fmap length_seq. lia.
+        - apply NoDup_fmap; last apply NoDup_seq.
+          apply Nat2Z.inj'.
+      }
+      iDestruct ("H'") as "(%s&Hl&%Hsize)".
+      iMod (token_alloc) as (γ) "Htoken".
+    iMod (inv_alloc (nroot) _
+            ( ∃ (tries':nat) (m:gmap nat _),
+                hashfun val_size f (<[LitLbl l:=fin_to_nat secret]> (kmap (λ x, LitInt (Z.of_nat x)) m))∗
+                lt ↦ #tries' ∗ (⌜(tries'<=tries)%nat ⌝) ∗
+                ((∃ (s':gset Z),
+                     (⌜∀ x y, m!!x=Some y -> y≠ fin_to_nat secret⌝) ∗
+                     ↯ (tries'/(val_size +1)%nat) ∗
+                     ↯ (tries' / size s') ∗
+                     ⌜secret_range + 1  + tries' - tries <=size s'⌝ ∗
+                     ⌜s' ## (set_map Z.of_nat (dom m):gset _)⌝ ∗
+                     l↪ urn_unif (s')
+                 )∨ (∃ x:Z,
+                        l↪ urn_unif {[x]}∗
+                        ⌜x∉((set_map Z.of_nat (dom m)):gset _)⌝ ∗
+                      token γ))
+            )%I
+           with "[Herr1 Hf Hr Hl]") as "#Hinv".
+    { iNext. iFrame "Hr".
+      iExists ∅.
+      rewrite kmap_empty.
+      iFrame.
+      iSplit; first done.
+      iLeft.
+      iFrame.
+      rewrite Rmult_plus_distr_l.
+      iDestruct (ec_split with "[$]") as "[Herr1 Herr2]".
+      { apply Rmult_le_pos; first apply pos_INR.
+        rewrite -!Rdiv_1_l.
+        apply Rcomplements.Rdiv_le_0_compat; try lra.
+        apply lt_0_INR; lia.  }
+      { apply Rmult_le_pos; first apply pos_INR.
+        rewrite -!Rdiv_1_l.
+        apply Rcomplements.Rdiv_le_0_compat; try lra.
+        apply lt_0_INR; lia.  }
+      rewrite !Rdiv_def.
+      rewrite Hsize. rewrite S_INR plus_INR.
+      replace 1%R with (INR 1) by done.
+      iFrame. 
+      repeat iSplit.
+      - iPureIntro.
+        intros. simplify_map_eq.
+      - iPureIntro. lia.
+      - rewrite dom_empty_L. rewrite set_map_empty. iPureIntro. set_solver.
+    }
+    
+    wp_bind (v _)%E.
+    rewrite refines_eq /refines_def.
+    simpl.
+    iApply (pgl_wp_wand); first iApply "Hinterp".
+    { iModIntro.
+      iIntros (?) "[%guess ->]".
+      rewrite refines_eq/refines_def.
+      wp_pures.
+      iInv "Hinv" as ">(%tries'&%m&Hf&Hl&%&Hor)" "Hclose".
+      wp_load.
+      wp_pures.
+      case_bool_decide.
+      - wp_pures.
+        iMod ("Hclose" with "[-]"); first by iFrame.
+        iModIntro.
+        iExists _. iLeft. by iSplit.
+      - wp_pures.
+        wp_load.
+        wp_pures.
+        wp_store.
+        iDestruct "Hor" as "[Hor|Hor]".
+        + (* normal case *)
+          admit.
+        + (* token case, its a weird case *)
+          iDestruct "Hor" as "(%x&Hu&%Hnotin&Htoken)".
+          destruct (decide (Z.of_nat guess =x)).
+          * subst.
+            wp_apply (wp_hashfun_prev _ _ _ _ _ _ _ (l↪ _) with "[$Hu $Hf]").
+            -- done.
+            -- by erewrite lookup_insert.
+            -- iSplit.
+               ++ iModIntro.
+                  iIntros.
+                  rewrite rupd_unseal/rupd_def.
+                  iIntros  (?) "[? Hu]". iSplit; last iFrame.
+                  iDestruct (ghost_map_lookup with "Hu [$]") as "%Hlookup".
+                  iPureIntro.
+                  intros.
+                  eapply urns_f_distr_lookup in Hlookup; last done; last done.
+                  destruct Hlookup as (?&Hsome&Hin).
+                  eexists _; split; last done.
+                  simpl.
+                  rewrite Hsome.
+                  simpl. rewrite bool_decide_eq_true_2; first done.
+                  set_solver.
+               ++ iModIntro.
+                  iApply big_sepS_intro.
+                  iModIntro.
+                  iIntros (?).
+                  rewrite elem_of_difference.
+                  iIntros ([H2 H3]) "?".
+                  rewrite rupd_unseal/rupd_def.
+                  iIntros  (?) "[? Hu]". iSplit; last iFrame.
+                  iDestruct (ghost_map_lookup with "Hu [$]") as "%Hlookup".
+                  iPureIntro.
+                  intros.
+                  eapply urns_f_distr_lookup in Hlookup; last done; last done.
+                  destruct Hlookup as (?&Hsome&Hin).
+                  eexists _; split; last done.
+                  simpl.
+                  rewrite elem_of_dom in H2.
+                  destruct H2.
+                  set_unfold. subst. simplify_map_eq.
+                  apply lookup_kmap_Some in H2; last (intros ???; by simplify_eq).
+                  destruct!/=. rewrite bool_decide_eq_false_2; first done.
+                  intros ?. simplify_eq.
+                  apply Hnotin.
+                  eexists _; split; first done.
+                  rewrite elem_of_dom. naive_solver.
+            -- iIntros "[Hf Hu]".
+               wp_pures.
+               iMod ("Hclose" with "[-]"); last first.
+               ++ iModIntro. iExists _. iRight.
+                  iSplit; first done.
+                  by iExists _.
+               ++ iNext.
+                  iExists _, _.
+                  replace (_-_)%Z with (Z.of_nat (tries' - 1)); last first. 
+                  { rewrite Nat2Z.inj_sub; first lia.
+                    destruct tries'; last lia.
+                    done. }
+                  iFrame "Hf Hl".
+                  iSplit; last iRight.
+                  ** iPureIntro. lia.
+                  ** by iFrame.
+          * destruct (decide (guess ∈ dom m)) as [H'|H'].
+            -- rewrite elem_of_dom in H'.
+               destruct H'.
+               wp_apply (wp_hashfun_prev _ _ _ _ _ _ (Z.of_nat guess) (l↪ _) with "[$Hu $Hf]").
+               ++ done.
+               ++ simplify_map_eq.
+                  apply lookup_kmap_Some; last naive_solver.
+                  intros ???. by simplify_eq.
+               ++ iSplit.
+                  ** iModIntro.
+                     iIntros.
+                     rewrite rupd_unseal/rupd_def.
+                     iIntros  (?) "[? Hu]". iSplit; last iFrame.
+                     iDestruct (ghost_map_lookup with "Hu [$]") as "%Hlookup".
+                     iPureIntro.
+                     intros.
+                     eapply urns_f_distr_lookup in Hlookup; last done; last done.
+                     destruct Hlookup as (?&Hsome&Hin).
+                     eexists _; split; last done.
+                     simpl. by rewrite bool_decide_eq_true_2.
+                  ** iModIntro.
+                     iApply big_sepS_intro.
+                     iModIntro.
+                     iIntros (?).
+                     rewrite elem_of_difference.
+                     iIntros ([K1 K2]) "?".
+                     rewrite rupd_unseal/rupd_def.
+                     iIntros  (?) "[? Hu]". iSplit; last iFrame.
+                     iDestruct (ghost_map_lookup with "Hu [$]") as "%Hlookup".
+                     iPureIntro.
+                     intros.
+                     eapply urns_f_distr_lookup in Hlookup; last done; last done.
+                     destruct Hlookup as (?&Hsome&Hin).
+                     eexists _; split; last done.
+                     simpl.
+                     rewrite elem_of_dom in K1.
+                     destruct K1 as [? K1].
+                     set_unfold. subst. simplify_map_eq.
+                     rewrite lookup_insert_Some in K1.
+                     destruct!/=.
+                     --- rewrite Hsome. simpl.
+                         rewrite bool_decide_eq_false_2; first done.
+                         intros ?. simplify_eq.
+                     --- rename select (kmap _ _ !! _ = _) into K1.
+                         apply lookup_kmap_Some in K1; last (intros ???; by simplify_eq).
+                         destruct!/=. rewrite bool_decide_eq_false_2; first done.
+                         intros ?. simplify_eq.
+               ++ iIntros "[Hf Hu]".
+               wp_pures.
+               iMod ("Hclose" with "[-]"); last first.
+                  ** iModIntro. iExists _. iRight.
+                     iSplit; first done.
+                     by iExists _.
+                  **  iNext.
+                      iExists _, _.
+                      replace (_-_)%Z with (Z.of_nat (tries' - 1)); last first. 
+                      { rewrite Nat2Z.inj_sub; first lia.
+                        destruct tries'; last lia.
+                        done. }
+                      iFrame "Hf Hl".
+                      iSplit; last iRight.
+                      --- iPureIntro. lia.
+                      --- by iFrame.
+            -- iMod (ec_zero) as "Hzero".
+               wp_apply (wp_insert_new _ _ _ _ _ _ (λ _, 0)%R (l↪ _) with "[$Hu $Hf $Hzero]").
+               ++ done.
+               ++ done.
+               ++ right. apply SeriesC_0. intros; lra.
+               ++ iModIntro.
+                  iApply big_sepS_intro.
+                  iModIntro.
+                  iIntros (?) "%Hlookup'".
+                  iIntros "?".
+                  rewrite rupd_unseal/rupd_def.
+                  iIntros  (?) "[? Hu]". iSplit; last iFrame.
+                  iDestruct (ghost_map_lookup with "Hu [$]") as "%Hlookup".
+                  iPureIntro.
+                  intros.
+                  eapply urns_f_distr_lookup in Hlookup; last done; last done.
+                  destruct Hlookup as (?&Hsome&Hin).
+                  eexists _; split; last done.
+                  simpl.
+                  rewrite elem_of_dom in Hlookup'.
+                  destruct Hlookup' as [? Hlookup'].
+                  rewrite lookup_insert_Some in Hlookup'.
+                  destruct!/=.
+                  --- rewrite Hsome/=. rewrite bool_decide_eq_false_2; first done.
+                      intros ?. simplify_eq.
+                      set_unfold. naive_solver.
+                  --- rename select (kmap _ _ !! _ = _) into K1.
+                      apply lookup_kmap_Some in K1; last (intros ???; by simplify_eq).
+                      destruct!/=. rewrite bool_decide_eq_false_2; first done.
+                      intros ?. simplify_eq.
+                      set_unfold. simplify_eq.
+                      rewrite elem_of_dom in H'. naive_solver.
+               ++ iIntros (?) "(Hf&Hurn&_)".
+                  rewrite insert_commute; last done.
+                  wp_pures.
+                  iMod ("Hclose" with "[-]"); last first.
+                  ** iModIntro. iExists _. iRight.
+                     iSplit; first done.
+                     by iExists _.
+                  **  iNext.
+                      iExists _, _.
+                      erewrite kmap_insert; last (intros ???; by simplify_eq).
+                      replace (_-_)%Z with (Z.of_nat (tries' - 1)); last first. 
+                      { rewrite Nat2Z.inj_sub; first lia.
+                        destruct tries'; last lia.
+                        done. }
+                      iFrame "Hf Hl".
+                      iSplit; last iRight.
+                      --- iPureIntro. lia.
+                      --- iFrame.
+                          iPureIntro.
+                          rewrite elem_of_map.
+                          intros ?. destruct!/=.
+                          set_solver.            
+    } 
+    iIntros (f') "#Hinterp'".
+    wp_bind (f' _)%E.
+    rewrite refines_eq /refines_def.
+    iApply (pgl_wp_wand); first iApply "Hinterp'".
+    { iExists (nat_to_fin _). by rewrite fin_to_nat_to_fin. }
+    iIntros (?) "[%guess ->]".
+    wp_pures.
+    admit.
+  Admitted.
+        
+End prog.
 
